.

src/Init/Data/Array/InsertionSort.lean
@@ -8,59 +8,88 @@ import Init.Data.Array.Basic
 import Init.Data.Nat.Fold
 import Init.Data.Vector.Lemmas
 
+namespace Vector
 
+/-- Swap the `i`-th element repeatedly to the left, while the element to its left is `lt` it. -/
+@[specialize, inline] def swapLeftWhileLT {n} (a : Vector α n) (i : Nat) (h : i < n)
+    (lt : α → α → Bool := by exact (· < ·)) : Vector α n :=
+  match h' : i with
+  | 0 => a
+  | i'+1 =>
+    if lt a[i'] a[i] then
+      swapLeftWhileLT (a.swap i' i) i' (by omega) lt
+    else
+      a
+
+end Vector
+
+open Vector
 namespace Array
 
+/-- Sort an array in place using insertion sort. -/
 @[inline] def insertionSort (a : Array α) (lt : α → α → Bool := by exact (· < ·)) : Array α :=
-  a.size.fold (init := ⟨a, rfl⟩) (f := fun i h acc => swapLoop acc i h) |>.toArray
-where
-  @[specialize] swapLoop {n} (a : Vector α n) (j : Nat) (h : j < n := by get_elem_tactic) : Vector α n :=
-    match h' : j with
-    | 0    => a
-    | j'+1 =>
-      if lt a[j] a[j'] then
-        swapLoop (a.swap j j') j'
-      else
-        a
+  a.size.fold (init := ⟨a, rfl⟩) (f := fun i h acc => swapLeftWhileLT acc i h lt) |>.toArray
 
 /-- Insert an element into an array, after the last element which is not `lt` the inserted element. -/
 def orderedInsert (a : Array α) (x : α) (lt : α → α → Bool := by exact (· < ·)) : Array α :=
-  insertionSort.swapLoop lt ⟨a.push x, rfl⟩ a.size (by simp) |>.toArray
+ swapLeftWhileLT ⟨a.push x, rfl⟩ a.size (by simp) lt |>.toArray
 
-@[simp] theorem size_insertionSort (a : Array α) : (a.insertionSort lt).size = a.size := by
-  simp [insertionSort]
+end Array
 
-theorem insertionSort_swapLoop_push {n} (a : Vector α n) (x : α) (j : Nat) (h : j < n) :
-    insertionSort.swapLoop lt (a.push x) j = (insertionSort.swapLoop lt a j).push x := by
+/-! ### Verification -/
+
+namespace Vector
+
+theorem swapLeftWhileLT_push {n} (a : Vector α n) (x : α) (j : Nat) (h : j < n) :
+    swapLeftWhileLT (a.push x) j (by omega) lt = (swapLeftWhileLT a j h lt).push x := by
   induction j generalizing a with
-  | zero => simp [insertionSort.swapLoop]
+  | zero => simp [swapLeftWhileLT]
   | succ j ih =>
-    simp [insertionSort.swapLoop]
+    simp [swapLeftWhileLT]
     split <;> rename_i h
     · rw [Vector.getElem_push_lt (by omega), Vector.getElem_push_lt (by omega)] at h
       rw [← Vector.push_swap, ih, if_pos h]
     · rw [Vector.getElem_push_lt (by omega), Vector.getElem_push_lt (by omega)] at h
       rw [if_neg h]
 
-theorem swapLoop_cast {n m} (a : Vector α n) (j : Nat) (h : j < n) (h : n = m) :
-    insertionSort.swapLoop lt (a.cast h) j = (insertionSort.swapLoop lt a j).cast h := by
-  subst h
+theorem swapLeftWhileLT_cast {n m} (a : Vector α n) (j : Nat) (h : j < n) (h' : n = m) :
+    swapLeftWhileLT (a.cast h') j (by omega) lt = (swapLeftWhileLT a j h lt).cast h' := by
+  subst h'
   simp
 
-theorem insertionSort_push (a : Array α) (x : α) :
+end Vector
+
+namespace Array
+
+@[simp] theorem size_insertionSort (a : Array α) : (a.insertionSort lt).size = a.size := by
+  simp [insertionSort]
+
+private theorem insertionSort_push' (a : Array α) (x : α) :
     (a.push x).insertionSort lt =
-      (insertionSort.swapLoop lt ⟨(a.insertionSort lt).push x, rfl⟩ a.size (by simp)).toArray := by
-  rw [insertionSort]
-  rw [Nat.fold_congr (size_push a x)]
-  rw [Nat.fold]
-  have : (a.size.fold (fun i h acc => insertionSort.swapLoop lt acc i (by simp; omega)) ⟨a.push x, rfl⟩) =
-      ((a.size.fold (fun i h acc => insertionSort.swapLoop lt acc i h) ⟨a, rfl⟩).push x).cast (by simp) := by
-    sorry
+      (swapLeftWhileLT ⟨(a.insertionSort lt).push x, rfl⟩ a.size (by simp) lt).toArray := by
+  rw [insertionSort, Nat.fold_congr (size_push a x), Nat.fold]
+  have : (a.size.fold (fun i h acc => swapLeftWhileLT acc i (by simp; omega) lt) ⟨a.push x, rfl⟩) =
+      ((a.size.fold (fun i h acc => swapLeftWhileLT acc i h lt) ⟨a, rfl⟩).push x).cast (by simp) := by
+    rw [Vector.eq_cast_iff]
+    simp only [Nat.fold_eq_finRange_foldl]
+    rw [← List.foldl_hom (fun a => (Vector.push x a)) _ (fun v ⟨i, h⟩ => swapLeftWhileLT v i (by omega) lt)]
+    rw [Vector.push_mk]
+    rw [← List.foldl_hom (Vector.cast _) _ (fun v ⟨i, h⟩ => swapLeftWhileLT v i (by omega) lt)]
+    · simp
+    · intro v i
+      simp only
+      rw [swapLeftWhileLT_cast]
+    · simp [swapLeftWhileLT_push]
   rw [this]
-  simp [swapLoop_cast]
+  simp only [Nat.lt_add_one, swapLeftWhileLT_cast, Vector.toArray_cast]
   unfold insertionSort
-  simp [Vector.push]
+  simp only [Vector.push]
   congr
   all_goals simp
+
+theorem insertionSort_push (a : Array α) (x : α) :
+    (a.push x).insertionSort lt = (a.insertionSort lt).orderedInsert x lt := by
+  rw [insertionSort_push', orderedInsert]
+  simp
 
 end Array
